Utils.v
@@ -1,9 +1,16 @@
 From Coq Require Import List.
 Import ListNotations.
+From Warblre Require Import Typeclasses.
 
-Fixpoint nth_opt {A: Type} (n: nat) (l: list A): option A :=
-  match n, l with
-  | _, nil => None
-  | 0, x::_ => Some x
-  | S n', _::q => nth_opt n' q
-  end.
+Module List.
+  Definition inb {A} `{EqDec A} (x: A) (l: list A): bool :=
+    if in_dec EqDec.eq_dec x l then true else false.
+
+  Lemma inb_spec {A} `{EqDec A}:
+    forall (x: A) (l: list A), inb x l = true <-> In x l.
+  Proof.
+    intros x l. unfold inb. destruct (in_dec _ x l).
+    - tauto.
+    - split. + discriminate. + contradiction.
+  Qed.
+End List.
